WIP

nondeterministic_dataflow/Timely_Operators.thy
@@ -6,42 +6,36 @@ imports
 begin
 
 datatype ('c, 'd) subgraph = 
-  "apply": Logic "'c \<Rightarrow> (nat, nat, 'd) op"
+  "apply": Logic "'c \<Rightarrow> 'c \<times> (nat, nat, 'd) op"
   | Seq "nat \<Rightarrow> 'd buf" "('c, 'd) subgraph" "('c, 'd) subgraph"
 
-
 inductive activate where
-  "step io (l c) (l' c') \<Longrightarrow> activate io c (Logic l) c' (Logic l')"
+  "l c = (c', op) \<Longrightarrow> l' c' = (_, op') \<Longrightarrow> step io op op' \<Longrightarrow> activate io c (Logic l) c' (Logic l')"
 | "activate (Out p x) c op1 c' op1' \<Longrightarrow>
    activate Tau c (Seq buf op1 op2) c' (Seq (BENQ p x buf) op1' op2)" 
- 
-(* friend_of_corec map_op where
-  "map_op f g (op :: ('i, 'o, 'd) op) = 
-  (case op of Silent op' \<Rightarrow> 
-    Silent (map_op f g op') 
-  | Write op' p x \<Rightarrow> Write (map_op f g op') (g p) x 
-  | Read p f' \<Rightarrow> Read (f p) (map_op f g o f')
-  | Choice ops \<Rightarrow> Choice (map_op f g |`| ops))"
- *)
-
-
 
 fun compile_subgraph where
   "compile_subgraph c (Logic l) = l c"
-| "compile_subgraph c (Seq buf sg1 sg2) = map_op projl projr (comp_op Some buf (compile_subgraph c sg1) (compile_subgraph c sg2))"
+| "compile_subgraph c (Seq buf sg1 sg2) = (
+  let (c', op1) = (compile_subgraph c sg1) in 
+  let (c'', op2) = (compile_subgraph c' sg2) in 
+  (c'', map_op projl projr (comp_op Some buf op1 op2)))"
 
 lemma
-  "activate io c t_op c' t_op' \<Longrightarrow>
-   step io (compile_subgraph c t_op) (compile_subgraph c' t_op')"
-  apply (induct io c t_op c' t_op' pred: activate)
-  subgoal for io op c op' c'
+  "activate io c t_op c'' t_op' \<Longrightarrow>
+   (c', op) = (compile_subgraph c t_op) \<Longrightarrow>
+   (c'', op') =  (compile_subgraph c' t_op') \<Longrightarrow>
+   step io op op'"
+  apply (induct io c t_op c'' t_op' arbitrary: op op' pred: activate)
+  subgoal for l c c' opa l' uu_ op'a io
     by simp
   subgoal for p x c op1 c' op1' buf op2
-    apply simp
+    apply (simp split: prod.splits)
       apply (rule step_map_op)
      apply simp_all
     apply (rule step_Tau_comp_op_L)
-    apply simp_all
+       apply simp_all
+   
 
       find_theorems comp_op Tau Out
 
